core/Syntax.v
@@ -24,8 +24,14 @@ Inductive OutputPatternElement : Type :=
   buildOutputPatternElement :
     (* id *) string 
     (* element expr *) -> (nat -> SourceModel -> (list SourceModelElement) -> option TargetModelElement) 
-    (* link expr *) -> ((SourceModel -> string -> list SourceModelElement -> nat -> option TargetModelElement) 
-                         -> nat -> SourceModel -> (list SourceModelElement) -> TargetModelElement -> option (list TargetModelLink)) -> OutputPatternElement.
+    (* link expr *) -> 
+      (** trace map *) ((SourceModel -> (list SourceModelElement * nat * string) -> option TargetModelElement) -> 
+      (** source model *) SourceModel -> 
+      (** source pattern *) (list SourceModelElement) -> 
+      (** iter *) nat ->
+      (** target model element *) TargetModelElement -> 
+      option (list TargetModelLink)) -> 
+        OutputPatternElement.
  
 Definition OutputPatternElement_getName (o: OutputPatternElement) : string :=
   match o with
